WIP qc

coq-minuska/theories/playground.v
@@ -1,18 +1,16 @@
 From Minuska Require Import
     prelude
     spec
+    specb
     default_static_model
     builtin.int_signature
     builtin.int_model
     pi.trivial
+    symex
 .
 
 From QuickChick Require Import QuickChick.
 Import QcDefaultNotation.
-
-
-
-(* Existing Instance int_model. *)
 
 #[local]
 Instance Σ : StaticModel := @default_model int_signature (int_model _ _ _) MyProgramInfo.
@@ -26,34 +24,149 @@ Definition genBuiltin : G builtin_value :=
     oneOf_ (returnGen (inl true)) [(returnGen (inl true)); (returnGen (inl false)); (returnGen (inr 1%Z));(returnGen (inr 2%Z))]
 .
 
-Sample genBuiltin.
-(* Print TermOver'. *)
-Fixpoint show_to (t : TermOver builtin_value) : string  :=
+Fixpoint show_to {T : Type} {_ST : Show T} (t : TermOver T) : string  :=
     match t with
     | t_over b => show b
-    | t_term s l => show s +:+ "(" +:+ (concat "," (show_to <$> l ))  +:+ ")"
+    | t_term s l => show s +:+ "[" +:+ (concat "," (show_to <$> l ))  +:+ "]"
     end
 .
 
 #[local]
-Instance showTerm : Show (TermOver builtin_value) := {|
+Instance showTerm {T : Type} {_ST : Show T} : Show (TermOver T) := {|
     show := show_to ;
 |}.
 
-Fixpoint genTermSized (sz : nat) : G (TermOver builtin_value) :=
+Definition genVariable : G variable :=
+    oneOf [ret "x"; ret "y"; ret "z"; ret "xx"; ret "yy"; ret "zz"]
+.
+
+Definition genSymbol : G symbol :=
+    (oneOf [(returnGen "s");(returnGen "t");(returnGen "a");(returnGen "b");(returnGen "c")])
+.
+
+Print IntFunSymbol.
+Compute builtin_function_symbol.
+
+Definition genFunction : G builtin_function_symbol :=
+    elems [int_plus; int_minus; int_uminus; int_zero; int_one; int_eq; int_le; int_lt]
+.
+
+Fixpoint genTermSized' {T : Type} (sz : nat) (g : nat -> G T) : G (TermOver T) :=
   match sz with
-    | O => bindGen genBuiltin (fun x => returnGen (t_over x))
+    | O => bindGen (g sz) (fun x => returnGen (t_over x))
     | S sz' =>
-        freq [ (1, bindGen genBuiltin (fun x => returnGen (t_over x))) ;
-                (sz, bindGen (oneOf_ (returnGen "") [(returnGen "s");(returnGen "t");(returnGen "a");(returnGen "b");(returnGen "c")])
-                (fun s => bindGen (listOf (genTermSized sz')) (fun l => returnGen (t_term s l))))
+        freq [ (1, bindGen (g sz) (fun x => returnGen (t_over x))) ;
+                (sz, bindGen genSymbol
+                (fun s => bindGen (listOf (genTermSized' sz' g)) (fun l => returnGen (t_term s l))))
              ]
   end.
 
+Definition genTermSized sz := genTermSized' sz (fun _ => genBuiltin).
+
+(* Print Expression2. *)
+
+#[local]
+Instance showFun : Show builtin_function_symbol := {|
+    show := fun f => match (f : builtin_function_symbol) with
+    | int_plus => "plus"
+    | int_minus => "minus"
+    | int_uminus => "uminus"
+    | int_zero => "zero"
+    | int_one => "one"
+    | int_eq => "eq"
+    | int_le => "le"
+    | int_lt => "lt"
+    end ;
+|}.
+
+#[local]
+Instance showQery : Show QuerySymbol := {|
+    show := fun q => match (q : QuerySymbol) with
+    | qs_program => "qs_program"
+    end ;
+|}.
 
 
-Locate forallb.
-(* Check returnGen. *)
-Sample (genTermSized 1).
+Fixpoint show_e (e : Expression2) : string  :=
+    match e with
+    | e_ground g => show g
+    | e_variable x => show x
+    | e_fun f l => show f +:+ "(" +:+ (concat "," (show_e <$> l ))  +:+ ")"
+    | e_query q l => show q +:+ "(" +:+ (concat "," (show_e <$> l ))  +:+ ")"
+    end
+.
+
+#[local]
+Instance showExpr : Show (Expression2) := {|
+    show := show_e ;
+|}.
 
 
+Fixpoint genExprSized (sz : nat) : G (Expression2) :=
+  match sz with
+    | O => oneOf [(bindGen genVariable (fun x => returnGen (e_variable x))); bindGen (genTermSized sz) (fun x => returnGen (e_ground x))]
+    | S sz' =>
+        freq [
+            (1,
+                oneOf [(bindGen genVariable (fun x => returnGen (e_variable x))); bindGen (genTermSized sz) (fun x => returnGen (e_ground x))]
+            );
+            (sz, 
+                bindGen (listOf (genExprSized sz')) (fun l =>
+                    bindGen (genFunction) (fun f =>
+                        ret (e_fun f l)
+                    )
+                )
+            )
+        ]
+  end.
+
+
+Definition genTermOverExprSized sz := genTermSized' sz genExprSized.
+
+Definition genValuationSized (sz : nat) : G (gmap variable (TermOver builtin_value)) :=
+    bindGen (
+        listOf (
+            bindGen genVariable (fun x =>
+                bindGen (genTermSized sz) (fun g =>
+                    returnGen (x, g)
+                )
+            )
+        )
+    ) (fun l => returnGen (list_to_map l))
+.
+
+#[local]
+Instance showVal : Show (gmap variable (TermOver builtin_value)) := {|
+    show := fun x => show (map_to_list x) ;
+|}.
+
+
+Sample (genValuationSized 2).
+(* Sample (genTermOverExprSized 3). *)
+
+Definition replace_and_collect_property
+    (program : ProgramT)
+    (g : TermOver builtin_value)
+    (et : TermOver Expression2)
+    (ρ : Valuation2)
+    (nv : NondetValue)
+    : Prop
+:=
+    sat2Eb program ρ g et nv =
+    sat2Bb ρ g (replace_and_collect et).1
+.
+
+QuickChick (
+    forAll
+        (genTermOverExprSized 3)
+        (
+            forAll
+                (genTermSized 3)
+                (
+                    forAll
+                        (genValSized 3)
+                        (replace_and_collect_property (t_over (inl false)))
+                )
+        )
+).
+(* replace_and_collect *)
