coq-minuska/theories/fresher.v
@@ -1,0 +1,68 @@
+From Minuska Require Import
+    prelude
+    spec
+.
+
+Record FresherR {Σ : StaticModel} := {
+    fresher_avoid : list variable ;
+}.
+
+Definition FresherM {Σ : StaticModel} (A : Type) : Type :=
+    FresherR -> (A*FresherR)%type
+.
+
+(* Definition fresherOf {Σ : StaticModel} (avoid : list variable)
+    : FresherM ()
+:=
+    fun _ => ((), {|fresher_avoid := avoid|})
+. *)
+
+Definition returnFresher {Σ : StaticModel}
+    {A : Type}
+    (a : A)
+    :
+    FresherM A
+:=
+    fun F => (a, F)
+.
+
+
+Definition fmapFresher
+    {Σ : StaticModel}
+    {A B : Type}
+    (f : A -> B)
+    (v : FresherM A)
+    : FresherM B
+:=
+    fun F =>
+    (f (v F).1, (v F).2)
+.
+
+
+Definition bindFresher
+    {Σ : StaticModel}
+    {A B : Type}
+    (v : FresherM A)
+    (f : A -> FresherM B)
+    : FresherM B
+:=
+    fun F =>
+    f (v F).1 F
+.
+
+
+Definition freshFresher
+    {Σ : StaticModel}
+    {A : Type}
+    (f : variable -> A)
+    : FresherM A
+:=
+    fun F =>
+    let x := fresh (F.(fresher_avoid)) in
+    let xs := x::(F.(fresher_avoid)) in
+    (f x, {|fresher_avoid:=xs;|})
+.
+
+
+
+
