coq-minuska/theories/symex.v
@@ -7,6 +7,7 @@ From Minuska Require Import
     unification_interface
     symex_spec
     valuation_merge
+    fresher
 .
 
 
@@ -17,6 +18,61 @@ Require Import Program.
 From Coq Require Import Logic.Eqdep_dec.
 
 From Equations Require Export Equations.
+
+
+Definition ScList {Σ : StaticModel} := (list (variable*(QuerySymbol+builtin_function_symbol)*(list (Expression2)))).
+
+(* To make sense, vars of F and vars of et should not overlap *)
+Fixpoint replace_and_collect0
+    {Σ : StaticModel}
+    (* (F : FresherM ()) *)
+    (et : (TermOver Expression2))
+    :
+    FresherM ((TermOver BuiltinOrVar)*ScList)
+:=
+    match et with
+    | t_over (e_ground g) => returnFresher (((TermOverBuiltin_to_TermOverBoV g)),[])
+    | t_over (e_variable x) => returnFresher ((t_over (bov_variable x)),[])
+    | t_over (e_fun f l) => 
+        freshFresher (fun x =>
+            (t_over (bov_variable x),[(x,(inr f), l)])
+        )
+    | t_over (e_query q l) => 
+        freshFresher (fun x =>
+            (t_over (bov_variable x),[(x,(inl q), l)])
+        )
+    | t_term s l => 
+        let a := (fix go (l : (list (TermOver Expression2))) : FresherM ((list (TermOver BuiltinOrVar))*ScList) :=
+            match l with
+            | nil => returnFresher (nil,nil)
+            | x::xs => bindFresher (replace_and_collect0 x) (
+                fun yr => bindFresher (go xs) (
+                    fun ysr => 
+                        let y := yr.1 in
+                        let r1 := yr.2 in
+                        let ys := ysr.1 in
+                        let r2 := ysr.2 in
+                        returnFresher ((y::ys), r1 ++ r2)
+                )
+            )
+            end
+        ) l in
+        (bindFresher a (fun b => returnFresher (t_term s b.1, b.2)))
+    end
+.
+
+Definition replace_and_collect
+    {Σ : StaticModel}
+    (et : (TermOver Expression2))
+    :
+    ((TermOver BuiltinOrVar)*ScList)
+:=
+    (replace_and_collect0 et {|fresher_avoid := (elements (vars_of et))|}).1
+.
+
+
+
+
 
 Module Implementation.
 
